reprove noskip and noreassign lemmas

src/Rupicola/Lib/Compiler.v
@@ -1,7 +1,7 @@
 Require Import Rupicola.Lib.Core.
 Require Import Rupicola.Lib.Notations.
 Require Import Rupicola.Lib.Tactics.
-Require Import coqutil.Tactics.fwd.
+Require Import bedrock2.Refinement.
 
 Section CompilerBasics.
   Context {width: Z} {BW: Bitwidth width} {word: word.word width} {memT: map.map word Byte.byte}.
@@ -273,42 +273,42 @@ Section with_parameters.
         + eapply Semantics.exec.seq; eassumption.
     Qed.
 
-    Definition refinement(c1 c2: cmd) := forall functions t m l post,
-        Semantics.exec.exec functions c1 t m l post ->
-        Semantics.exec.exec functions c2 t m l post.
-
-    Lemma use_refinement_while: forall functions test body1 body2,
-        refinement body1 body2 ->
-        forall t m l post,
-        Semantics.exec.exec functions (cmd.while test body1) t m l post ->
-        Semantics.exec.exec functions (cmd.while test body2) t m l post.
-    Proof.
-      intros * R *. remember (cmd.while test body1) as c1. intros. revert Heqc1.
-      induction H; intros; subst; inversion Heqc1; subst.
-      - eapply Semantics.exec.while_false; eassumption.
-      - eapply Semantics.exec.while_true; try eassumption.
-        { unfold refinement in R.
-          eapply R. eassumption. }
-        intros.
-        eapply H3; eauto.
-    Qed.
-
     Lemma noskips_correct_bw:
-      forall cmd {tr mem locals functions} post,
+      forall cmd {functions tr mem locals} post,
         Semantics.exec functions (noskips cmd) tr mem locals post ->
         Semantics.exec functions cmd tr mem locals post.
     Proof.
-      induction cmd; cbn in *; intros;
-        repeat match goal with
-          | H: _ = noskips _ |- _ => discriminate H
-          end;
-        cbn in *;
-        fwd;
+      induction cmd; intros;
+        match goal with
+        | H: Semantics.exec.exec _ (noskips ?c) _ _ _ _ |- _ =>
+            lazymatch c with
+            | cmd.while _ _ => idtac
+            | cmd.seq _ _ => idtac
+            | _ => inversion H; clear H; subst
+            end
+        end;
         try solve [econstructor; eauto].
-      8: {
-        eapply use_refinement_while. 2: exact H.
+      { cbn in *. destruct (is_skip (noskips cmd1)) eqn: E1.
+        { eapply is_skip_sound in E1.
+          eapply Semantics.exec.seq.
+          { eapply IHcmd1. rewrite E1.
+            eapply Semantics.exec.skip with
+              (post := fun t m l => t = tr /\ m = mem /\ l = locals).
+            auto. }
+          cbv beta. intros * (? & ? & ?); subst.
+          eapply IHcmd2. assumption. }
+        destruct (is_skip (noskips cmd2)) eqn: E2.
+        { eapply is_skip_sound in E2.
+          eapply Semantics.exec.seq.
+          { eapply IHcmd1. eassumption. }
+          intros. eapply IHcmd2. rewrite E2. eapply Semantics.exec.skip. assumption. }
+        inversion H. subst.
+        eapply Semantics.exec.seq.
+        { eapply IHcmd1. eassumption. }
+        { intros. eapply IHcmd2. eauto. } }
+      { cbn in *. eapply refinement_while. 2: exact H.
         unfold refinement. intros *. eapply IHcmd. }
-    Admitted.
+    Qed.
 
     Lemma noskips_correct:
       forall cmd {tr mem locals functions} post,
@@ -317,45 +317,10 @@ Section with_parameters.
         WeakestPrecondition.program functions
           cmd tr mem locals post.
     Proof.
-      split; revert tr mem locals post.
-      all: induction cmd;
-        repeat match goal with
-               | _ => eassumption
-               | _ => apply IHcmd
-               | [ H: _ /\ _ |- _ ] => destruct H
-               | [  |- _ /\ _ ] => split
-               | [ H: forall v t m l, ?P v t m l -> exists _, _ |- ?P _ _ _ _ -> _ ] =>
-                 let h := fresh in intros h; specialize (H _ _ _ _ h)
-               | [ H: exists _, _ |- _ ] => destruct H
-               | [  |- exists _, _ ] => eexists
-               | [ H: context[WeakestPrecondition.cmd] |- context[WeakestPrecondition.cmd] ] => solve [eapply H; eauto]
-               | _ => unfold WeakestPrecondition.program in * || cbn || intros ? || eauto
-               end.
-    Admitted.
-    (*
-      2: {
-        eapply Loops.wp_while.
-
-      all: try (destruct (is_skip (noskips cmd1)) eqn:H1;
-        [ apply is_skip_sound in H1; rewrite H1 in * |
-          apply is_skip_complete in H1;
-           (destruct (is_skip (noskips cmd2)) eqn:H2;
-            [ apply is_skip_sound in H2; rewrite H2 in * |
-              apply is_skip_complete in H2 ]) ]).
-
-      - apply IHcmd1, IHcmd2; eassumption.
-      - eapply WeakestPrecondition_weaken, IHcmd1; eauto.
-      - eapply WeakestPrecondition_weaken.
-        * intros * H0. eapply IHcmd2. apply H0.
-        * eapply IHcmd1. eassumption.
-
-      - eapply IHcmd1 in H. eapply IHcmd2. eassumption.
-      - eapply IHcmd1 in H. eapply WeakestPrecondition_weaken in H; [ apply H |].
-        intros; eapply IHcmd2; eauto.
-      - apply IHcmd1 in H. eapply WeakestPrecondition_weaken in H; [ apply H |].
-        intros * H0%IHcmd2. apply H0.
+      unfold program. split; intros.
+      - eapply complete_cmd. eapply sound_cmd in H. eapply noskips_correct_bw. assumption.
+      - eapply complete_cmd. eapply sound_cmd in H. eapply noskips_correct_fw. assumption.
     Qed.
-    *)
 
     Definition compile_setup_remove_skips := noskips_correct.
 
@@ -420,7 +385,11 @@ Section with_parameters.
         rewrite map.put_idemp in H0; assumption.
       - eapply WeakestPrecondition_weaken, IHcmd1; eauto;
           intros; eapply WeakestPrecondition_weaken, IHcmd2; eauto.
-    Admitted.
+      - eapply WP.WP_Impl.mk_wp_cmd. eapply WP.WP_Impl.invert_wp_cmd in H.
+        eapply refinement_while. 2: eassumption.
+        unfold refinement. intros.
+        eapply sound_cmd. eapply IHcmd. eapply complete_cmd. assumption.
+    Qed.
 
     Definition compile_setup_remove_reassigns := noreassign_correct.
     Strategy 1 [noreassign is_var_expr].
